Partial progress in DecodeTapes

theories/TM/Code/Decode.v
@@ -1,25 +1,28 @@
 From Undecidability.TM Require Import TM Code.
 
 Import Retracts.
+
+Class Encode_prefixInjective (sig: Type) (X: Type) (cX : codable sig X) := {
+  encode_prefixInjective : forall (x x' :X) t t', encode x ++ t = encode x' ++ t' -> x = x'
+}.
+
 Module ContainsEncoding.
   Section containsEncoding.
     Local Unset Implicit Arguments.
 
     Context {sig tau:Type} {n:nat} {X:Type}.
-    Context (cX : codable sig X) (f : sig -> tau).
+    Context (encode : X -> list sig) (f : sig -> tau).
     (*Hypothesis (nonEmpty : forall x, encode x <> []).*)
 
     Definition Rel : pRel tau bool 1 :=
       fun tin '(yout, tout) =>
         match yout with
           true => exists (x:X) t__L t__R,
-                 let t__x := map f (encode x) in
-                 (exists c__hd, hd_error t__x = Some c__hd /\  tin[@Fin0] = midtape t__L c__hd (tl t__x++t__R) )
-                 /\ exists c__last, hd_error (rev t__x) = Some c__last /\ tout[@Fin0] = midtape (tl(rev t__x)++ t__L) c__last t__R
+                 (exists x__hd x__tl, encode x = x__hd::x__tl /\  tin[@Fin0] = midtape t__L (f x__hd) (map f x__tl++t__R) )
+                 /\ exists x__init x__last , encode x = x__init ++ [x__last] /\ tout[@Fin0] = midtape (map f (rev x__init)++ t__L) (f x__last) t__R
         | false => forall t__L (x:X) t__R,
-            let t__x := map f (encode x) in
-            exists c__hd, hd_error t__x = Some c__hd /\
-            tin[@Fin0] <> midtape t__L c__hd (tl t__x++t__R)
+            exists x__hd x__tl, map f (encode x) = x__hd::x__tl /\ 
+            tin[@Fin0] <> midtape t__L x__hd (x__tl++t__R)
         end.
   End containsEncoding.
 End ContainsEncoding.
