theories/TM/Single/DecodeTapes.v
@@ -2,14 +2,16 @@ From Undecidability.TM Require Import TM ProgrammingTools Code.Decode Code Singl
 Require Import Lia Ring Arith Program.Wf.
 Import While Mono Multi Switch If Combinators EncodeTapes.
 
-
+Unset Printing Coercions.
 From Coq.ssr Require ssrfun.
 Module Option := ssrfun.Option.
 
 Module CheckEncodeTapes.
   Section checkEncodeTapes.
 
-    Context (sig: Type).
+    (* This actually checks for the encoding of lists of a given. *)
+
+    Context (sig: finType).
 
     Context (tau:finType) `{I : Retract (sigList (sigTape sig)) tau}.
 
@@ -20,92 +22,60 @@ Module CheckEncodeTapes.
     
     Definition Rel n : pRel tau bool 1 := ContainsEncoding.Rel (Encode_tapes sig n) Retr_f.
     
-    Compute encode [ 2 : nat;3].
+    Fixpoint R_syntactic n (t: tape tau) (b:bool) t' : Prop :=
+        match n with
+          0   => inhabited (reflect (Option.bind Retr_g (current t) = Some sigList_nil) b) /\ t = t'
+        | S n => (Option.bind Retr_g (current t) = Some sigList_cons
+                 /\ exists t1 b1, ContainsEncoding.Rel (Encode_tape sig) Retr_f [|tape_move_right t|] (b1,t1)
+                            /\ if b1 then R_syntactic n (tape_move_right t1[@Fin0]) b t'
+                              else t1[@Fin0]=t' /\ b = false)
+                \/ (Option.bind Retr_g (current t) <> Some sigList_cons /\ b = false)
+        end.
 
-    Local Definition isList_nil {sig} (c:sigList sig) := match c with sigList_nil => true | _ => false end.
-    Local Definition isList_cons {sig} (c:sigList sig) := match c with sigList_cons => true | _ => false end.
-
-
-    Definition f__step t : bool * tape tau :=
-      if (Option.apply isList_cons false (Option.bind Retr_g (current t)))
-               then let r := CheckEncodesTape.f (I:=I__X) (tape_move_right t) in
-                    if fst r then (true,tape_move_right (snd r)) else (false,snd r)
-               else (false,t).
-
-    Fixpoint f n t {struct n}: bool * tape tau :=
-      match n with
-        0 => (Option.apply isList_nil false (Option.bind Retr_g (current t)),t)
-      | S i => let r := f__step t in
-              if fst r then f i (snd r) else r
-      end.
-
-    Local Hint Rewrite map_map : list.
-    
-    Lemma f_spec n t b t':
-      f n t = (b,t')
+    Lemma R_syntactic__spec n t b t':
+      R_syntactic n t b t'
       -> Rel n [|t|] (b,[|t'|]).
     Proof.
-      induction n in t|-*;cbn.
-      -intros [= <- <-]. destruct Option.apply eqn:Hc.
-       +destruct Option.bind eqn:Hc'. 2:easy. destruct s;inv Hc. 
-        destruct (current t) eqn:Hc. 2:easy. apply retract_g_inv in Hc' as ->.
-        destruct t;inv Hc.
-        eexists [||],_,_. split. all:eexists _;cbn. all:easy.
-       +intros ? v ?. rewrite (destruct_vector_nil v);cbn. eexists;split;[easy | ]. intros ->;cbn in Hc. now retract_adjoint.
-      -remember (f__step _) as res eqn:Hres;revert Hres. unfold f__step.
-       destruct Option.apply eqn:Hc.
-       2:{ clear IHn. intros -> [= <- <-];cbn. intros ? v ?. specialize (destruct_vector_cons v) as (t0&v'&->). cbn.
-           do 2 eexists. easy. intros ->. cbn in Hc. destruct t0;cbn in Hc. all:retract_adjoint;cbn in *. all:easy.
-       }
-       edestruct CheckEncodesTape.f as [b' t''] eqn:Hf. apply CheckEncodesTape.f_spec in Hf. hnf in Hf.
-       destruct b';cbn.
-       2:{ clear IHn. intros -> [= <- <-]. intros ? v ?. specialize (destruct_vector_cons v) as (t0&v'&->);cbn.
-           do 2 eexists. easy. intros ->. cbn in Hc;retract_adjoint. cbn in *;inv Hc.
-           destruct (encode_tape t0) eqn: Ht0. now destruct t0.  
-           edestruct Hf with (x:=t0) as (?&?&?);cbn in *. rewrite Ht0 in *. inv H. 
-           apply H0. f_equal. unfold retr_comp_f. cbn. now autorewrite with list. 
-       }
-       cbn in Hf. destruct Hf as (t0&t__L0&t__R0&[(?&Hhd&Ht) (?&Htl&->)]).
-       destruct rev eqn: eqHtl in Htl;inv Htl. destruct map eqn: eqHhd in Hhd;inv Hhd. 
-       destruct t as [ | | | t__L c__t t__R]. 1-3:easy.
-       revert Ht. destruct t__R. easy.  intros [= <- <- ->]. cbn in Hc.
-       (destruct (Retr_g c__t) as [[] | ] eqn:Hc__t';inv Hc);[]. apply retract_g_inv in Hc__t' as ->.
-       unfold retr_comp_f in *.
-       (* cbn in *. 
-       destruct (encode_tape t0)  eqn:eqt0 in Hhd,Ht. now destruct t0. cbn in Hhd,Ht. unfold retr_comp_f in Hhd. inv Hhd. 
-        *)
-       intros -> [= Hres]. specialize IHn with (1:= Hres).
-       cbn in IHn.  destruct b. unfold encode_tapes in *.
-       +destruct IHn as (ts&?&t__R&[(?&Hhd'&Ht1) (?&Htl'&->)]).
-        destruct rev eqn: eqHtl' in Htl';inv Htl'. destruct map eqn: eqHhd' in Hhd';inv Hhd'. 
-        revert Ht1. destruct t__R0;cbn. easy. intros [= <- <- -> ].
-        eexists (t0:::ts), _, t__R. cbn. autorewrite with list.
-        rewrite eqHtl',eqHtl,eqHhd',eqHhd. cbn. repeat (autorewrite with list;cbn).
-        repeat esplit.
-       +intros t__L' v t__R'. specialize (destruct_vector_cons v) as (t0'&v'&->);cbn. do 2 eexists. easy.
-        autorewrite with list. rewrite eqHhd. cbn. change (e :: l0 ++ t__R0) with ((e :: l0) ++ t__R0). rewrite <- eqHhd.
-         intros [= <- H']. revert H'. (*Error???*)
-         (* TODO: *)revert H'. destruct (vector_to_list v');cbn.
-         all:autorewrite with list. all:set (c := map _ _). set (c':=map _ _). all:try length_not_eq.  rdestruct (map Retr_f (encode_tapes x)) eqn:Hx. now destruct x.
-         destruct x.  Set Printing All. autorewrite with list.
-        edestruct IHn as (c__hd&Hc__hd&Ht).  cbn in *. cbn in Ht. easy. destruct IHn as 
-        destruct rev eqn: eqHtl' in Htl';inv Htl'. destruct map eqn: eqHhd' in Hhd';inv Hhd'. 
-        revert Ht1. destruct t__R0;cbn. easy. intros [= <- <- -> ].
-        eexists (t0:::ts), _, t__R. cbn. autorewrite with list.
-        rewrite eqHtl',eqHtl,eqHhd',eqHhd. cbn. repeat (autorewrite with list;cbn).
-        repeat esplit.
-        *rewrite eqdestruct (encode_list (Encode_tape sig) (vector_to_list ts)) eqn:eqhd'. now inv Hhd'. inv Hhd'.
-         repeat eexists. rewrite eqt0;cbn;autorewrite with list. now repeat f_equal.
-        *destruct (rev _) eqn:eqhd' in Htl'. now inv Htl'. inv Htl'.
-         destruct (rev _) eqn:eqtl in Htl. now inv Htl. inv Htl.
-         rewrite eqt0 in *;cbn in *;autorewrite with list. do 2 eexists. 2:f_equal.
-         all:rewrite eqhd';cbn. easy. autorewrite with list.
-         destruct rev eqn:eqtl' in eqtl;cbn in eqtl.
-         { inv eqtl. destructeqtl. cbn. congruence. easy. repeat f_equal. cbn. 
-         repeat eexists.  2:repeat f_equal.
-       
-       
-           destruct x;cbn in *. 
+      unfold Rel. unfold encode,Encode_tapes,encode_tapes. 
+      induction n in t |-*;cbn [R_syntactic].
+      {unfold Rel, ContainsEncoding.Rel. intros [[Hb] <-]. destruct Hb.
+       -destruct t;inv e. apply retract_g_inv in H0 as ->.
+        eexists [||],_,_. cbn. split. now eexists _,[]. now eexists [],_.
+       -intros ? v ?. rewrite (destruct_vector_nil v);cbn.
+        eexists _,_. split. easy. intros ->. cbn in n. now retract_adjoint.
+      }
+      intros [(Ht&t1&b1&HR&Hb1) | (Ht&->)].
+      2:{ clear IHn. cbn in *. intros ? v ?. destruct (destruct_vector_cons v) as (t0&b'&->). cbn.
+          do 3 eexists. reflexivity. intros ->. cbn in Ht. now retract_adjoint. }
+      cbn. destruct b1;hnf in HR. 
+      2:{ clear IHn. destruct Hb1 as [<- ->]. intros ? v ?. destruct (destruct_vector_cons v) as (t0&b'&->). cbn.
+          do 3 eexists. easy. intros ->. cbn in HR.
+          edestruct HR with (x:=t0) as (?&?&Hhd&Henc).
+          destruct (encode_tape t0) eqn:Ht0. all:inv Hhd. cbn in Henc.
+          apply Henc. unfold retr_comp_f. cbn. autorewrite with list. rewrite map_map. reflexivity. }
+      cbn in HR. revert Ht. destruct t as [ | | | t__L c t__R];intros [= ->%retract_g_inv].
+      destruct HR as (t0&t__L'&t__R'&(x__hd&x__tl&eq__hd&Ht)&(x__init&x__last&eq__last&Ht')). rewrite Ht' in Hb1. clear t1 Ht'.
+      destruct t__R; inv Ht. cbn in Hb1. specialize IHn with (1:=Hb1);cbn in IHn.
+      destruct b.
+      -destruct IHn as (v&t__Lv&t__Rv&(x__hd'&x__tl'&eq__hd'&Ht)&(x__init'&x__last'&eq__last'&->)).
+       destruct t__R' as [ |? t__R'];inv Ht. eexists (t0:::v),_,_;split.
+       +cbn. do 3 eexists. reflexivity. rewrite eq__hd, eq__hd'. unfold retr_comp_f. cbn;autorewrite with list;cbn. rewrite map_map. easy.
+       +cbn. rewrite eq__last, eq__last'. unfold retr_comp_f. cbn;autorewrite with list;cbn.
+        eexists (_::_++_::_),_. split. 1:{ repeat (cbn;autorewrite with list). easy. }
+        f_equal. repeat (cbn;autorewrite with list;try rewrite map_rev;try rewrite map_map). easy.
+      -intros ? v ?. destruct (destruct_vector_cons v) as (t0'&b'&->). cbn.
+       do 3 eexists. reflexivity. intros [= <- H]. revert H. unfold retr_comp_f;autorewrite with list;rewrite map_map.
+       rewrite app_comm_cons,<-(map_cons (fun a : sigTape sig => Retr_f (sigList_X a))). rewrite <- eq__hd.
+       intros H. assert (H':=H). change (fun x : sigTape sig => Retr_f  (sigList_X x)) with (Retr_f) in H'.
+       eapply (f_equal (map _)) in H'. rewrite !map_app,!(surject_inject' _ NilBlank) in H'. 
+       change (@encode_tape sig) with (encode (X:=tape sig)) in H'.
+       apply (encode_prefixInjective (X:=tape sig)) in H'. subst t0'.
+       apply app_inv_head in H as ->. 
+       edestruct IHn as (?&?&?&Hneq). apply Hneq. cbn. rewrite H. cbn.
+       f_equal.
+    Qed.
+
+    (*
     Definition M__step : pTM tau (option bool) 1 :=
       Switch ReadChar
           (fun x =>
@@ -121,7 +91,7 @@ Module CheckEncodeTapes.
 
     Definition M' (bs : bool*bool) := 
       StateWhile M__step bs.
-
-  End checkEncodeList.
-End CheckEncodeList.
-*)
+     *)
+    
+  End checkEncodeTapes.
+End CheckEncodeTapes.
