theories/TM/Single/DecodeTape.v
@@ -1,15 +1,47 @@
 From Undecidability.TM Require Import TM ProgrammingTools Code.Decode.
 
-From Undecidability.TM Require Single.EncodeTapes Single.StepTM Single.EncodeTapesInvariants.
+From Undecidability.TM Require Single.EncodeTapes Single.StepTM Single.EncodeTapesInvariants .
 Require Import FunInd Lia Ring Arith Program.Wf.
+Import EncodeTapes EncodeTapesInvariants.
 
 From Coq.ssr Require ssrfun.
 Module Option := ssrfun.Option.
+From Coq Require ssreflect ssrfun ssrbool.
 
+Section wlog.
+  (*Import ssreflect ssrfun ssrbool.
+  Set Implicit Arguments.
+  Unset Strict Implicit.
+  Unset Printing Implicit Defensive.*)
+  Global Instance tape_encode_prefixInjective sig: Encode_prefixInjective (Encode_tape sig).
+  Proof.
+    (** General Idea: encode_tape_invariants can be used to show equal length
+    Then we could prove a lemma that it suffices that the dame symbol is marked and tape_to_list is the same or something... *)
+    
+    (*econstructor.
+    unfold encode;cbn.
+    intros x x'.
+    wlog: x x' / (length (encode_tape x) <= length (encode_tape x')).
+    {intros H. decide (length (encode_tape x) <= length (encode_tape x')). now apply H.
+     intros. symmetry. eapply H. nia. now setoid_rewrite H0. }
+    intros Hle t t' H.
+    specialize encode_tape_invariants with (t0:=x) as [-> | (b__L&b__R&t__x&Hx&Hsymb__x&Hmark__x&neq__x)]. now destruct x';inv H.
+    specialize encode_tape_invariants with (t0:=x') as [-> | (b__L'&b__R'&t__x'&Hx'&Hsymb__x'&Hmark__x'&neq__x')]. now destruct x;inv H.
+(* TODO: 
+-may eb seperate invariants into seperat lemmas?*)
+    
+    (*assert (Hfst := f_equal (firstn (| encode_tape x |)) H). assert (Hskip := f_equal (skipn (| encode_tape x |)) H).
+    rewrite firstn_all2 with (l:=)
+    
+    
+    ssreflect.ssr_wlog *) *)
+  Admitted.
+End wlog.
+    
 Module CheckEncodesTape.
   Section checkEncodesTape.
 
-    Import EncodeTapes StateWhile Mono Multi Copy Switch If Combinators Single.EncodeTapesInvariants.
+    Import Mono Multi Copy Switch If Combinators.
     
     Context (sig : Type) (tau:finType) {I : Retract (sigTape sig) tau}.
 
@@ -32,6 +64,7 @@ Module CheckEncodesTape.
                else Return (Move R) (inl (haveSeenMark || isMarked c,haveSeenSymbol || isSymbol c))
              end).
 
+    (** We can do it as function here, althought that is not the prefered way. Instead, just define a "pretty" version o the relation you realise, then you don;t have to worry about termination *)
     Definition f__step bs t : (bool * bool + bool) * tape tau :=
       let (haveSeenMark,haveSeenSymbol) := (fst bs,snd bs) in
       match Option.bind Retr_g (current t) with
@@ -181,13 +214,13 @@ Module CheckEncodesTape.
       ->  if fst res then
            exists (x:tape sig) t__R1 (t__R2 : list tau) c',
              t__R = map Retr_f t__R1++t__R2
-             /\ Some c' = Retr_g c
+             /\ c = Retr_f c'
              /\ encode_tape x = LeftBlank b :: rev t__L'++c'::t__R1
              /\ snd res = midtape (tail (rev (map Retr_f t__R1)++[c])++map Retr_f (t__L'++[LeftBlank b])++t__L) (hd c (rev (map Retr_f t__R1)++[c])) t__R2
          else
            forall x t__R1 (t__R2 : list tau) c',
              t__R = map Retr_f t__R1++t__R2 ->
-             Some c' = Retr_g c ->
+             c = Retr_f c' ->
              encode_tape x <> LeftBlank b :: rev t__L'++c'::t__R1.
     Proof.
       rewrite map_app;cbn.
@@ -198,61 +231,66 @@ Module CheckEncodesTape.
       destruct (Retr_g c) as [ [] | ] eqn:Hgc ;cbn. 1-3,6:clear IH.
       -replace (fst res) with false.
        2:{ destruct marked;cbn in Hf. destruct seenMark in Hf;cbn in Hf. all:now subst. }
-       clear - H__symbs.
-       intros ? ? ? ? -> [= ->] (Hneq&Hsym&(?&Hlast)&_)%encode_tape_invariants_partial;cbn in *. 2:now setoid_rewrite <- in_rev.
-       destruct t__R1. easy. discriminate (Hsym (LeftBlank marked)). rewrite tl_app. 2:now length_not_eq. now eauto.     
+       clear Hf Hres. 
+       intros ? ? ? ? -> [= ->] ((init__R&b__R&H__R&Hsym)&Hmarks&Hlength)%encode_tape_invariants_partial;cbn in *. 2:now setoid_rewrite <- in_rev.
+       retract_adjoint. inv Hgc. destruct init__R;inv H__R.  ediscriminate (Hsym (LeftBlank _)). easy.     
       -cbn in Hf. rewrite !orb_true_r in Hf. subst f. revert Hres. 
        destruct marked;cbn in *. destruct seenMark;cbn in *. all:intros ->;cbn. 3:destruct seenMark;cbn. 2,3:destruct seenSymbol;cbn.
-       +intros ? ? ? ? -> [= ->] (Hneq&Hsym&(?&Hlast)&Hmarks)%encode_tape_invariants_partial;cbn in *. 2:now setoid_rewrite <- in_rev.
-        autorewrite with list in *. nia.
+       +intros ? ? ? ? -> [= ->] ((init__R&b__R&H__R&Hsym)&Hmarks&Hlength)%encode_tape_invariants_partial;cbn in *. 2:now setoid_rewrite <- in_rev.
+        retract_adjoint. inv Hgc. cbn in Hmarks;autorewrite with list in *. nia.
        +edestruct invert_symbols_0_marked with (t:= t__L') as (t__R2&->).
         1,2:autorewrite with list in *. now nia. now intros;eapply H__symbs.
         destruct b. 1:{exfalso. autorewrite with list in H__seenMark. now cbn in H__seenMark;nia. } 
-        destruct t__R2 as [ | c' cs] eqn:Htp. 1:{exfalso. inversion H__seenSymbol. easy. } 
+        destruct t__R2 as [ | c' cs] eqn:Htp. 1:{exfalso. inversion H__seenSymbol. easy. }
+        apply retract_g_inv in Hgc as ->.
         eexists (rightof _ _),[],_,_. repeat eapply conj. 1,2,4:reflexivity. cbn.
         autorewrite with list;cbn.  setoid_rewrite <- map_rev with (l:=cs) at 2. easy.
-       +intros ? ? ? ? -> [= ->] (Hneq&Hsym&(?&Hlast)&Hmarks&Hnempty)%encode_tape_invariants_partial;cbn in *.
-        2:now setoid_rewrite <- in_rev.
+       +intros ? ? ? ? -> [= ->] ((init__R&b__R&H__R&Hsym)&Hmarks&Hlength)%encode_tape_invariants_partial;cbn in *. 2:now setoid_rewrite <- in_rev.
+        retract_adjoint. inv Hgc.
         destruct t__L'. all:inv H__seenSymbol. 2:now apply H. cbn in *;autorewrite with list in *.
-        destruct t__R1. 2:{ ediscriminate (Hsym (RightBlank _)). rewrite tl_app. eauto. length_not_eq. }
+        destruct init__R;inv H__R. 2:{ ediscriminate (Hsym (RightBlank _)). easy. }
         cbn in *. nia.
        +destruct b.
         *edestruct invert_symbols_0_marked with (t:= t__L') as (t__R2&->).
          1,2:autorewrite with list in *;cbn in *. now nia. now intros;eapply H__symbs.
          destruct t__R2 eqn:?. 1:{exfalso. inversion H__seenSymbol. easy. }
-         destruct (rev t__R2) eqn:Htp. 1:{exfalso. subst. revert Htp. length_not_eq. } 
+         destruct (rev t__R2) eqn:Htp. 1:{exfalso. subst. revert Htp. length_not_eq. }
+          apply retract_g_inv in Hgc as ->.
          eexists (leftof _ _),[],_,_. repeat eapply conj. 1,2,4:reflexivity. rewrite <- Heql. cbn.
          setoid_rewrite <- map_rev with (l:=t__R2). now rewrite Htp.
         *edestruct @invert_symbols_1_marked with (t:= t__L') as (?&?&?&->).
          1,2:autorewrite with list in *;cbn in *. now nia. now intros;eapply H__symbs.
+         apply retract_g_inv in Hgc as ->.
          eexists (midtape _ _ _),[],_,_. repeat eapply conj. 1,2,4:reflexivity. cbn.
          repeat (autorewrite with list;cbn).  setoid_rewrite map_rev. easy.
-       +intros ? ? ? ? -> [= -> ] (Hneq&Hsym&(?&Hlast)&Hmarks&?)%encode_tape_invariants_partial;cbn in *.
-        2:now setoid_rewrite <- in_rev.
-        destruct t__R1. 2:{ ediscriminate (Hsym (RightBlank _)). rewrite tl_app. 2:now length_not_eq. eauto. }
-        destruct t__L'. 2:{ inversion H__seenSymbol. now apply H. }
-        cbn in *. nia.
-       +intros ? ? ? ? -> [= ->] (Hneq&Hsym&(?&Hlast)&Hmarks&?)%encode_tape_invariants_partial;cbn in *.
-        2:now setoid_rewrite <- in_rev.
-        destruct t__R1. 2:{ ediscriminate (Hsym (RightBlank _)). rewrite tl_app. 2:now length_not_eq. eauto. }
+       +intros ? ? ? ? -> [= -> ] ((init__R&b__R&H__R&Hsym)&Hmarks&Hlength)%encode_tape_invariants_partial;cbn in *.
+        2:now setoid_rewrite <- in_rev. retract_adjoint. inv Hgc.
+        destruct init__R;inv H__R. 2:{ ediscriminate (Hsym (RightBlank _)). easy. }
+        cbn in *. assert (t__L' = []) as ->. 1:{ destruct t__L'. easy. inversion H__seenSymbol. destruct H. easy. }
+        cbn in *;nia.
+       +intros ? ? ? ? -> [= ->] ((init__R&b__R&H__R&Hsym)&Hmarks&Hlength)%encode_tape_invariants_partial;cbn in *.
+        2:now setoid_rewrite <- in_rev. retract_adjoint. inv Hgc. 
+        destruct init__R;inv H__R. 2:{ ediscriminate (Hsym (RightBlank _)). easy. }
         cbn in *. autorewrite with list in *. nia.
       -replace (fst res) with false.
        2:{ cbn in Hf. destruct seenMark in Hf;cbn in Hf. all:now subst. }
-       clear - H__symbs.
-       intros ? ? ? ? -> [= -> ] (Hneq&Hsym&(?&Hlast)&_)%encode_tape_invariants_partial;cbn in *. 2:now setoid_rewrite <- in_rev.
-       destruct t__R1. easy. discriminate (Hsym (NilBlank)). rewrite tl_app. 2:now length_not_eq. now eauto.   
-      -subst f res;cbn. easy.
+       clear Hf Hres. 
+       intros ? ? ? ? -> [= ->]((init__R&b__R&H__R&Hsym)&Hmarks&Hlength)%encode_tape_invariants_partial;cbn in *. 2:now setoid_rewrite <- in_rev.
+        retract_adjoint. inv Hgc.
+       destruct init__R;inv H__R. discriminate (Hsym (NilBlank)). easy.   
+      -subst f res;cbn. intros ? ? ? ? _ ->. edestruct (retract_g_None Hgc). easy.
       -revert Hf Hres. cbn. destruct seenMark;cbn.
        {clear IH. intros -> ->;cbn.
-        intros ? ? ? ? -> [= ->](Hneq&Hsym&(?&Hlast)&?&?)%encode_tape_invariants_partial;cbn in *. 2:now setoid_rewrite <- in_rev.
-        cbn in *. autorewrite with list in *. nia.
+        intros ? ? ? ? -> [= ->]((init__R&b__R&H__R&Hsym)&Hmarks&Hlength)%encode_tape_invariants_partial;cbn in *. 2:now setoid_rewrite <- in_rev.
+        retract_adjoint. inv Hgc. cbn in *.
+        autorewrite with list in *. nia.
        } intros ->;cbn.
        destruct t__R.
        { clear IH. cbn. rewrite f'_equation;cbn.  
          intros ->;cbn.
-         intros ? ? ? ? Hnil [= ->] (Hneq&Hsym&(?&Hlast)&?&?)%encode_tape_invariants_partial;cbn in *.
-         2:now setoid_rewrite <- in_rev.
-         destruct t__R1. 2:easy. destruct t__R2. 2:easy. easy.
+         intros ? ? ? ? Hnil [= ->] ((init__R&b__R&H__R&Hsym)&Hmarks&Hlength)%encode_tape_invariants_partial;cbn in *.
+         2:now setoid_rewrite <- in_rev. retract_adjoint. inv Hgc.
+         destruct init__R;inv H__R. length_not_eq in Hnil. 
        }
        cbn. intros H.
        autorewrite with list in H__seenMark. destruct b;cbn in H__seenMark. now nia. 
@@ -261,22 +299,25 @@ Module CheckEncodesTape.
        3:reflexivity. 2:nia. 2:now autorewrite with list in *;nia. 2:now intros ? [<- | ];eauto.
        2:now rewrite orb_true_r;constructor.
        destruct res as [[] t'];cbn in *.
-       +destruct H' as (x&t__R1&t__R2&c'&->&Hc'&Hx&->).
+       +destruct H' as (x&t__R1&t__R2&c'&->&->&Hx&->).
         eexists x,(_::t__R1),t__R2,_.
-        repeat (cbn in Hx|-*;autorewrite with list in Hx|-* ). erewrite <- retract_g_inv. 2:symmetry;eassumption.
+        repeat (cbn in Hx|-*;autorewrite with list in Hx|-* ).
+        apply retract_g_inv in Hgc as ->.
         split. 2:split. 3:split.
         1,2:reflexivity. easy.
         destruct (rev (map Retr_f t__R1));cbn;now autorewrite with list.
-       +intros x ? ? ? H__R [= ->] Hx. specialize encode_tape_invariants_partial with (1:=Hx) as (Hneq&Hsym&(?&Hlast)&_);cbn in *. now setoid_rewrite <- in_rev.
-        destruct (rev t__R1) eqn:Heq. all:inv Hlast.
-        destruct t__R1. now inv Heq. inv H__R. eapply H'. reflexivity.  now rewrite retract_g_adjoint.
-        rewrite Hx;cbn;autorewrite with list;cbn. reflexivity.
+       +intros x ? ? ? H__R [= ->] Hx. specialize encode_tape_invariants_partial with (1:=Hx) as ((init__R&b__R&H__R'&Hsym)&Hmarks&Hlength);cbn in *. now setoid_rewrite <- in_rev.
+        retract_adjoint. inv Hgc.
+        destruct init__R;inv H__R'.
+        destruct (init__R ++ [RightBlank b__R]) eqn:eq. now length_not_eq in eq. revert H__R;intros [= -> ->].
+        eapply H'. 1,2:easy. rewrite Hx;cbn;autorewrite with list;cbn. reflexivity.
       -revert Hf Hres. cbn. intros ->;cbn.
        destruct t__R.
        { clear IH. cbn. rewrite f'_equation;cbn.  
          intros ->;cbn.
-         intros ? ? ? ? Hnil [= ->] (Hneq&Hsym&(?&Hlast)&?&?)%encode_tape_invariants_partial;cbn in *.
-         2:now setoid_rewrite <- in_rev.  destruct t__R1. 2:easy. destruct t__R2. 2:easy. easy.
+         intros ? ? ? ? Hnil [= ->] ((init__R&b__R&H__R&Hsym)&Hmarks&Hlength)%encode_tape_invariants_partial;cbn in *.
+         retract_adjoint. inv Hgc. 
+         2:now setoid_rewrite <- in_rev.  destruct t__R1. 2:easy. destruct init__R.  2:length_not_eq in H__R. inv H__R. 
        }
        cbn;intros H.
        specialize IH with (t__L' := UnmarkedSymbol s :: t__L');cbn in IH. erewrite <- !(retract_g_inv Hgc) in IH.
@@ -284,13 +325,16 @@ Module CheckEncodesTape.
        3:reflexivity. 2:lia. 3:now intros ? [<- | ];eauto. 3:now rewrite orb_true_r;constructor.
        2:{ autorewrite with list in *. destruct seenMark;cbn in *;nia. }
        destruct res as [[] t'];cbn in *.
-       +destruct H' as (x&t__R1&t__R2&c'&->&Hc&Hx&->).
-        eexists x,(_::t__R1),t__R2,_. cbn.  erewrite <- retract_g_inv. 2:symmetry;eassumption.
+       +destruct H' as (x&t__R1&t__R2&c'&->&->&Hx&->).
+        apply retract_g_inv in Hgc as ->. 
+        eexists x,(_::t__R1),t__R2,_. cbn.
         repeat (cbn in Hx|-*;autorewrite with list in Hx|-* ). split. 2:split. 3:split. 1,2:reflexivity. easy.
         destruct (rev (map Retr_f t__R1));cbn;now autorewrite with list.
-       +intros x ? ? ? H__R [= ->] Hx. specialize encode_tape_invariants_partial with (1:=Hx) as (Hneq&Hsym&(?&Hlast)&_);cbn in *. now setoid_rewrite <- in_rev.
-        destruct (rev t__R1) eqn:Heq. all:inv Hlast.
-        destruct t__R1. now inv Heq. inv H__R. eapply H'. 1:reflexivity. 1:now rewrite retract_g_adjoint. rewrite Hx;cbn;autorewrite with list;cbn. reflexivity.
+       +intros x ? ? ? H__R [= ->] Hx. specialize encode_tape_invariants_partial with (1:=Hx) as ((init__R&b__R&H__R'&Hsym)&Hmarks&Hlength);cbn in *. now setoid_rewrite <- in_rev.
+        retract_adjoint. inv Hgc.
+        setoid_rewrite <- app_assoc in H'. cbn in H'.
+        destruct t__R1;inv H__R. 1:{ destruct init__R. easy. length_not_eq in H__R'. }
+        eapply H'. 1,2:reflexivity. now rewrite Hx.
     Qed.
 
     Lemma f_spec t b t':
@@ -298,29 +342,36 @@ Module CheckEncodesTape.
       -> Rel [|t|] (b,[|t'|]).
     Proof.
       unfold f;cbn. destruct Option.bind eqn:Hcur.
-      2:{ intros [= <- <-];cbn;intros ? ? ?. destruct x;cbn;eexists;(split;[reflexivity| ]). all:intros ->;cbn in Hcur. all:now rewrite retract_g_adjoint in Hcur. }
+      2:{ intros [= <- <-];cbn;intros ? ? ?. destruct x;cbn;eexists _,_;(split;[reflexivity| ]). all:intros ->;cbn in Hcur. all:now rewrite retract_g_adjoint in Hcur. }
       destruct t as [ | | | t__L s' t__R];cbn in *. 1-3:now inversion Hcur.
       apply retract_g_inv in Hcur as ->. 
       destruct isLeftBlank eqn:H__LB.
       2:destruct isNilBlank eqn:H__NB.
-      2:{ intros [= <- <- ]. destruct s;inv H__NB. eexists (@niltape _),_,_;cbn. eauto 10. }
-      2:{ intros [= <- <- ]. intros ? x ?. destruct x;cbn;eexists;(split;[reflexivity | ]).
+      2:{ intros [= <- <- ]. destruct s;inv H__NB. eexists (@niltape _),t__L,t__R;cbn.
+          split. eexists _, nil;cbn. easy. eexists nil,_;cbn. easy. }
+      2:{ intros [= <- <- ]. intros ? x ?. destruct x;cbn;eexists _,_;(split;[reflexivity | ]).
           all:intros [= <- ->%retract_f_injective ->]. all:easy. }
       destruct s;inv H__LB.
-      destruct t__R. 1:{ cbn. rewrite f'_equation. cbn. intros [= <- <-]. intros ? x ?. destruct x;cbn;eexists;(split;[reflexivity | ]). all:intros [= <- ?%retract_f_injective ?]. easy. all:revert H0. all:length_not_eq. }
+      destruct t__R. 1:{ cbn. rewrite f'_equation. cbn. intros [= <- <-]. intros ? x ?.
+                       destruct x;cbn;eexists _,_;(split;[reflexivity | ]). all:intros [= <- ?%retract_f_injective ?]. easy. all:revert H0. all:length_not_eq. }
       intros H';symmetry in H'. assert (H:=H'). revert H. intros H%(f'_spec (t__L':=[])).
       2:now destruct marked;cbn;nia. 2:easy. 2:now constructor. destruct b;cbn  in H.
-      -destruct H as (x&t__R1&t__R2&c'&->& ->%eq_sym%retract_g_inv &Hx&->). all:destruct ((rev (map Retr_f (encode_tape x)))) eqn:Hlast.
-       1:{ rewrite Hx in Hlast. exfalso;revert Hlast; length_not_eq. }
-       do 5 eexists.
-       +rewrite Hx;cbn. eauto.
-       +setoid_rewrite Hlast at 1. rewrite Hx in Hlast. cbn in Hlast.
-        apply (f_equal (hd (Retr_f c'))) in Hlast. cbn in Hlast. rewrite hd_app in Hlast. 2: length_not_eq.
-        rewrite Hlast.  rewrite Hx. cbn. rewrite <- !tl_app. 2,3:length_not_eq. repeat (autorewrite with list;cbn). eauto 10.
-      -intros ? x ?. eexists (hd (Retr_f NilBlank) (map Retr_f (encode_tape x))). split. now destruct x.
-       intros [= <- H1 H2]. destruct encode_tape eqn:Heqt. all:apply retract_f_injective in H1. now inv H1. cbn in *. subst s.
-       destruct l. 1:{ destruct x;cbn in Heqt;try now inv Heqt. all:revert Heqt. all:length_not_eq. }
-       inv H2. eapply H. reflexivity. 2:exact Heqt. now rewrite retract_g_adjoint.
+      -destruct H as (x&t__R1&t__R2&c'&->& -> &Hx&->).
+       eexists _,_,_;split.
+       +rewrite Hx;cbn. do 3 eexists. easy. cbn. eauto.
+       +destruct (exists_last (l:=encode_tape x)) as (?&?&eqx). congruence. rewrite eqx in *.
+        repeat eexists.
+        apply (f_equal (fun t => rev (map Retr_f t))) in Hx. cbn in  Hx.
+        autorewrite with list in Hx;cbn in Hx. f_equal.
+        
+        *rewrite (app_comm_cons' _ _ (Retr_f (LeftBlank marked))). rewrite <- tl_app. 2: length_not_eq.
+         rewrite <- app_assoc. cbn. rewrite <- Hx. cbn. now rewrite map_rev.
+        *apply (f_equal (hd (Retr_f c'))) in Hx. destruct rev;cbn in *. all: easy.
+      -intros ? x ?.
+       destruct encode_tape eqn:eqx. now destruct x.
+       do 3 eexists. cbn. easy. intros [= <- <-%retract_f_injective H''].
+       destruct l. 1:{ destruct x;cbn in eqx;try now inv eqx. all:length_not_eq in eqx. }
+       inv H''. eapply H. 1,2:reflexivity. eassumption.
     Qed.
 
   End checkEncodesTape.
