theories/TM/Single/EncodeTapesInvariants.v
@@ -20,7 +20,8 @@ Lemma encode_tape_invariants sig t0 :
   t0 = (@niltape _)
   \/ exists b__L b__R t, encode_tape t0 = LeftBlank b__L :: t ++[RightBlank b__R]
                /\ (forall x, x el t -> isSymbol x = true)
-               /\ length (filter (@isMarked sig) (encode_tape t0)) = 1.
+               /\ length (filter (@isMarked sig) (encode_tape t0)) = 1
+               /\ t <> nil.
 Proof.
   assert (H' : forall l x, x el map UnmarkedSymbol l -> (@isSymbol sig) x = true).
   { intros ? ? (?&<-&?)%in_map_iff. easy. }
@@ -32,7 +33,7 @@ Proof.
   all:split;[cbn;autorewrite with list;reflexivity | ].
   all:cbn in *;repeat setoid_rewrite in_app_iff;cbn. all:split;[now intuition (subst;eauto 3) | ].
   all:repeat (repeat rewrite map_rev;autorewrite with list;cbn).
-  all:repeat rewrite H1'. all:now cbn.
+  all:repeat rewrite H1'. all:split;[easy | ]. all:now length_not_eq.
 Qed.
 
 
@@ -40,31 +41,27 @@ Qed.
 Lemma encode_tape_invariants_partial sig (x:tape sig) b t t__R:
   encode_tape x = LeftBlank b :: t ++t__R
   -> (forall x, x el t  -> isSymbol x = true)
-  -> t__R <> []
-    /\ (forall c , c el tail (rev t__R) -> isSymbol c = true)
-    /\ (exists b', head (rev t__R) = Some (RightBlank b'))
-    /\ (length (filter (@isMarked _) (t__R++t++[LeftBlank b])) = 1)
-    /\ length (t++t__R) > 1.
+  -> (exists init__R b',
+      t__R = init__R++[RightBlank b']
+      /\ (forall c , c el init__R -> isSymbol c = true))
+      /\ (length (filter (@isMarked _) (t__R++t++[LeftBlank b])) = 1)
+      /\ length (t++t__R) > 1.
 Proof.
-  destruct (encode_tape_invariants x) as [-> | (b__L&b__R&t'&Hx&Hsymb&Hmarked)].
+  destruct (encode_tape_invariants x) as [-> | (b__L&b__R&t'&Hx&Hsymb&Hmarked&Hnnil)].
   {cbn;congruence. }
   rewrite Hx. intros [= <- Ht'] Hall.
-  destruct t__R eqn:Ht__R in |-. 1:{ subst. rewrite app_nil_r in Ht'. subst t. ediscriminate (Hall (RightBlank _)). now eauto. }
-  split. now congruence.
-  destruct (rev t__R) eqn: H__rev. 1:{ subst t__R. length_not_eq in H__rev. }
-  cbn in *.
-  rewrite <- rev_involutive with (l:=t__R) in Ht'. rewrite H__rev in Ht';cbn in Ht'.
-  rewrite app_assoc in Ht'. apply Prelim.last_app_eq in Ht' as (->&<-).        
-  split. 2:split. 3:split.
-  -setoid_rewrite in_app_iff in Hsymb. setoid_rewrite <- in_rev in Hsymb. eauto.
-  -eauto.
-  -apply (f_equal (@rev _)) in H__rev. rewrite rev_involutive in H__rev.  rewrite H__rev. cbn.
-   rewrite Hx in Hmarked. cbn in *.  autorewrite with list in *;cbn in *.
-   destruct b__L,b__R;cbn in *. all:autorewrite with list in *;cbn in *. all:nia.
-  -subst t__R. destruct t. 2:now autorewrite with list;cbn;nia.
-   cbn in *. destruct l. 2:cbn;nia.
-   inv H__rev.
-   destruct x;inv Hx. all: length_not_eq in H1. 
+  assert (H__R : t__R <> []). 1:{ destruct t__R. 2:easy. rewrite app_nil_r in Ht'. subst t. ediscriminate (Hall (RightBlank _)). now eauto. }
+  apply exists_last in H__R as (init__R&last__R&->). 
+  rewrite !app_assoc in Ht';apply Prelim.last_app_eq in Ht' as [-> [= <-]]. 
+  split. 1:{ eexists _, _;split. reflexivity. intros. apply Hsymb. eauto. }
+  destruct x;cbn in Hx,Hmarked;autorewrite with list in Hmarked,Hx;revert Hx. easy.
+  all:intros [= <- H];revert H.
+  2:rewrite (app_comm_cons' _ _ (UnmarkedSymbol _)).
+  all:rewrite ?app_comm_cons, <- !app_assoc_reverse. all:intros [H <-]%Prelim.last_app_eq;revert H.
+  all:intros H%(f_equal (fun l => length (filter (isMarked (sig:=sig)) l) )).
+  all:repeat (autorewrite with list in Hmarked,H|-*;cbn in Hmarked,H|-* ).
+  all:split;[ | now destruct t;[destruct init__R| ];cbn in *;try congruence;nia].
+  all:nia.
 Qed.
 
 Lemma invert_symbols_0_marked sig t:
